progs/verif_message.v
@@ -520,6 +520,9 @@ unfold SeparationLogic.maybe_retval.
 change (fun rho : environ =>
     serialize_post msg (v, p, buf, sh_p, sh_buf) (get_result1 x rho))
  with (`(serialize_post msg (v, p, buf, sh_p, sh_buf)) (get_result1 x)).
+simpl @snd.
+change(maybe_retval (serialize_post msg (v, p, buf, sh_p, sh_buf)) tint (Some x))
+  with (`(serialize_post msg (v, p, buf, sh_p, sh_buf)) (get_result1 x)).
 autorewrite with subst.
 go_lowerx. normalize.
 unfold serialize_post, serialize_spec.
