Makefile
@@ -19,7 +19,7 @@ COMPCERT=compcert
 CC_TARGET=compcert/cfrontend/Clight.vo
 CC_DIRS= lib common cfrontend exportclight
 DIRS= msl sepcomp veric floyd progs sha linking compcomp
-INCLUDE= $(foreach a,$(DIRS), -I $(a) -as $(a)) -R $(COMPCERT) -as compcert
+INCLUDE= $(foreach a,$(DIRS),$(if $(wildcard $(a)), -I $(a) -as $(a))) -R $(COMPCERT) -as compcert
 # $(foreach a,$(CC_DIRS), -R $(COMPCERT)/$(a) -as compcert.$(a)) -I $(COMPCERT)/flocq -as compcert.flocq
 
 CV1=$(shell cat compcert/VERSION)
